cava/cava/Cava/Arrow/ArrowKind.v
@@ -1,0 +1,182 @@
+(****************************************************************************)
+(* Copyright 2020 The Project Oak Authors                                   *)
+(*                                                                          *)
+(* Licensed under the Apache License, Version 2.0 (the "License")           *)
+(* you may not use this file except in compliance with the License.         *)
+(* You may obtain a copy of the License at                                  *)
+(*                                                                          *)
+(*     http://www.apache.org/licenses/LICENSE-2.0                           *)
+(*                                                                          *)
+(* Unless required by applicable law or agreed to in writing, software      *)
+(* distributed under the License is distributed on an "AS IS" BASIS,        *)
+(* WITHOUT WARRANTIES OR CONDITIONS OF ANY KIND, either express or implied. *)
+(* See the License for the specific language governing permissions and      *)
+(* limitations under the License.                                           *)
+(****************************************************************************)
+
+From Coq Require Import Lists.List NaryFunctions Arith NArith Vector Eqdep_dec.
+
+Import ListNotations.
+Import VectorNotations.
+
+From Cava Require Import Types.
+
+Inductive Kind : Set :=
+| Tuple: Kind -> Kind -> Kind
+| Unit: Kind
+| Bit: Kind
+| Vector: Kind -> nat -> Kind.
+
+Fixpoint eq_kind_dec (k1 k2: Kind) {struct k1} : {k1=k2} + {k1<>k2}.
+Proof.
+  decide equality.
+  exact (PeanoNat.Nat.eq_dec n n0).
+Defined.
+
+(* TODO: Coq.Init.Logic f_equal2 is opaque, f_equal is not, should transparency here be upstreamed? *)
+Lemma f_equal2 {A B C} {x y:A}  {a b: B} (f: A -> B -> C) : x = y -> a = b -> f x a = f y b.
+Proof.
+  destruct 1.
+  destruct 1.
+  trivial.
+Defined.
+
+Definition kind_proj_tup_left (ty: Kind):=
+  match ty with
+  | Tuple t1 t2 => t1
+  | _ => ty
+  end.
+
+Definition kind_proj_tup_right (ty: Kind):=
+  match ty with
+  | Tuple t1 t2 => t2
+  | _ => ty
+  end.
+Definition kind_proj_vec_t (ty: Kind):=
+  match ty with
+  | Vector t _ => t
+  | _ => ty
+  end.
+Definition kind_proj_vec_n (ty: Kind) :=
+  match ty with
+  | Vector _ n => n
+  | _ => 0
+  end.
+
+Lemma UIP_refl_kind (ty:Kind) (x : ty = ty) : x = eq_refl.
+Proof.
+  induction ty.
+
+  - specialize IHty1 with (f_equal kind_proj_tup_left x).
+    specialize IHty2 with (f_equal kind_proj_tup_right x).
+    change eq_refl with (f_equal2 Tuple (@eq_refl _ ty1) (@eq_refl _ ty2)).
+    rewrite <- IHty1.
+    rewrite <- IHty2.
+    clear IHty1.
+    clear IHty2.
+
+    change (match Tuple ty1 ty2 as x return Tuple ty1 ty2 = x -> Prop with
+            | Tuple _ _ =>
+              fun H => H = f_equal2 Tuple (f_equal kind_proj_tup_left H) (f_equal kind_proj_tup_right H)
+            | _ => fun _ => True
+            end x).
+    pattern (Tuple ty1 ty2) at 2 3, x.
+    destruct x.
+    reflexivity.
+
+  - change (match Unit as n return Unit=n -> Prop with
+            | Unit => fun x => x = eq_refl
+            | _ => fun _ => True
+            end x); destruct x; reflexivity.
+
+  - change (match Bit as n return Bit=n -> Prop with
+            | Bit => fun x => x = eq_refl
+            | _ => fun _ => True
+            end x); destruct x; reflexivity.
+
+  - specialize IHty with (f_equal kind_proj_vec_t x).
+    pose proof (UIP_refl_nat n (f_equal kind_proj_vec_n x)).
+    change eq_refl with (f_equal2 Vector (@eq_refl _ ty) (@eq_refl _ n)).
+    rewrite <- IHty.
+    rewrite <- H.
+    clear IHty.
+    clear H.
+    change (match Vector ty n as a return Vector ty n = a -> Prop with
+            | Vector _ _ => fun x => x = f_equal2 Vector (f_equal kind_proj_vec_t x) (f_equal kind_proj_vec_n x)
+            | _ => fun _ => True
+            end x).
+
+    pattern (Vector ty n) at 2 3, x.
+    destruct x.
+    reflexivity.
+Defined.
+
+
+Lemma kind_eq: forall ty, eq_kind_dec ty ty = left eq_refl.
+Proof.
+  intros.
+  destruct (eq_kind_dec ty ty); try rewrite (UIP_refl_kind _ _); auto.
+  destruct n.
+  reflexivity.
+Qed.
+
+Ltac reduce_kind_eq :=
+  match goal with
+  | [ |- context[eq_kind_dec _ _] ] =>
+    rewrite kind_eq; unfold eq_rect_r, eq_rect, eq_sym
+  | [H: context[eq_kind_dec _ _] |- _] =>
+    rewrite kind_eq in H; unfold eq_rect_r, eq_rect, eq_sym in H
+  end; try subst.
+
+Declare Scope kind_scope.
+Bind Scope kind_scope with Kind.
+
+Notation "<< x >>" := (x) : kind_scope.
+Notation "<< x , .. , y , z >>" := (Tuple x .. (Tuple y z )  .. ) : kind_scope.
+
+Fixpoint arg_length (ty: Kind) :=
+match ty with
+| Tuple _ r => S (arg_length r)
+| _ => O
+end.
+
+Definition arg_length_order (ty1 ty2: Kind) :=
+  arg_length ty1 < arg_length ty2.
+
+Lemma arg_length_order_wf': forall len ty, arg_length ty < len -> Acc arg_length_order ty.
+Proof.
+  unfold arg_length_order; induction len; intros.
+  - inversion H.
+  - refine (Acc_intro _ _); intros.
+    eapply (IHlen y).
+
+    apply lt_n_Sm_le in H.
+    apply (lt_le_trans _ _ _ H0 H).
+Defined.
+
+Lemma arg_length_order_wf: well_founded arg_length_order.
+Proof.
+  cbv [well_founded]; intros.
+  eapply arg_length_order_wf'.
+  eauto.
+Defined.
+
+Fixpoint vec_to_nprod (A: Type) n (v: Vector.t A n): A^n :=
+  match v with
+  | [] => tt
+  | x::xs => (x, vec_to_nprod A _ xs)
+  end%vector.
+
+Fixpoint insert_rightmost_unit (ty: Kind): Kind :=
+match ty with
+| Tuple l r => Tuple l (insert_rightmost_unit r)
+| Unit => Unit
+| x => Tuple x Unit
+end.
+
+Fixpoint remove_rightmost_unit (ty: Kind): Kind :=
+match ty with
+| Tuple l Unit => l
+| Tuple l r => Tuple l (remove_rightmost_unit r)
+| x => x
+end.
